spec/prop/vfmDecreasesGasScript.sml
@@ -1473,7 +1473,7 @@ Theorem step_create_lemma:
         ; data     := []
         (* unused: for concreteness *)
         ; nonce := 0; gasPrice := 0; accessList := []
-        ; blobGasPrice := 0; blobVersionedHashes := []
+        ; blobVersionedHashes := []
       |>;
       rollback <- get_rollback;
       _ <- update_accounts $
